Evaluation rewrote with an inductive predicate + In EvalP, a inductive predicate `evalP` is shown equivalent to the big step evaluator + PartialMonotonicity, Compatibility, Stackability and Wellformedness rewrote to use `evalP` + Stackability and Local Reasonning not done yet.

src/PartialMonotonicity.v
@@ -2,7 +2,7 @@
 (* Clément Blaudeau - LAMP@EPFL 2021 *)
 (** This file defines the notion of partial monotonicity between stores. The idea behind partial monotonicity is simple: objects that are being initialized (not warm already) can only get "warmer": the number of initialized fields can only increase. Between two stores [σ] and [σ'], it means that all objects in [σ] have more initialized fields in [σ']; it does not states anything about new objects that [σ'] can have. *)
 
-From Celsius Require Export Trees Eval Reachability Tactics Compatibility strongInduction.
+From Celsius Require Export Compatibility.
 Require Import ssreflect ssrbool List Psatz Coq.Program.Tactics.
 Import ListNotations.
 Open Scope nat_scope.
@@ -15,25 +15,36 @@ Definition initializedFields σ l (f: list Field) : Prop :=
   end.
 Notation "σ ⊨ l : f" := (initializedFields σ l f) (at level 80, l at level 80, f at level 80).
 
-Definition partialMonotonicity (σ σ': Store) :=
+Definition partialMonotonicity σ σ' :=
   forall l f, (σ ⊨ l : f) -> (σ' ⊨ l : f).
 Notation "σ ⪯ σ'" := (partialMonotonicity σ σ') (at level 80).
+#[global] Hint Unfold partialMonotonicity: pM.
+
 
 (** ** Basic results *)
 (** The relation is trivially reflexive *)
-Lemma partialMonotonicity_reflexivity :
+Lemma pM_refl:
   forall σ, σ ⪯ σ.
 Proof.
-  unfold partialMonotonicity => //.
+  auto with pM.
 Qed.
-Global Hint Resolve partialMonotonicity_reflexivity: pM.
+#[global] Hint Resolve pM_refl: pM.
 
 (** The relation is trivially transitive *)
-Lemma partialMonotonicity_transitivity : forall (σ1 σ2 σ3 : Store), (σ1 ⪯ σ2) -> (σ2 ⪯ σ3) -> (σ1 ⪯ σ3).
+Lemma pM_trans : forall σ1 σ2 σ3, (σ1 ⪯ σ2) -> (σ2 ⪯ σ3) -> (σ1 ⪯ σ3).
 Proof.
-  unfold partialMonotonicity; auto.
+  auto with pM.
 Qed.
-Global Hint Resolve partialMonotonicity_transitivity: pM.
+#[global] Hint Resolve pM_trans: pM.
+
+Ltac pM_trans :=
+  repeat match goal with
+         | H:_ |- ?σ ⪯ ?σ => apply pM_refl
+         | H: ?σ1 ⪯ ?σ2 |- ?σ1 ⪯ ?σ3 => apply pM_trans with σ2 ; [ assumption | ]
+         | H: ?σ2 ⪯ ?σ3 |- ?σ1 ⪯ ?σ3 => apply pM_trans with σ2 ; [ | assumption ]
+         end.
+#[global] Hint Extern 1 => pM_trans: pM.
+
 
 (** Initialized fields are within the domain *)
 Lemma initializedFields_dom :
@@ -52,34 +63,33 @@ Lemma initializedFields_exists :
   exists f, ((c,e)::σ) ⊨ (dom σ) : f.
 Proof.
   unfold initializedFields.
-  intros. exists [].
+  intros. exists ([]: list Field).
   induction σ; intros ; simpl ; try lia.
   - destruct σ, a; steps; lia.
 Qed.
 Global Hint Resolve initializedFields_exists: pM.
 
 (** We have a result on the store sizes *)
-Lemma partialMonotonicity_domains:
+Lemma pM_domains:
   forall σ σ',
     σ ⪯ σ' -> dom σ <= dom σ'.
 Proof.
   unfold partialMonotonicity; intros.
   destruct σ eqn:Σ; simpl; [lia |].
   destruct o.
-  case : (initializedFields_exists s c e) => f Hf.
+  case : (initializedFields_exists l c e) => f Hf.
   eauto using Lt.lt_le_S with pM.
 Qed.
-Global Hint Resolve partialMonotonicity_domains: pM.
+Global Hint Resolve pM_domains: pM.
 
 
 (** ** Main Monotonicity result *)
 (** We start with two technical results on partial monotonicity for assignment (update) and fresh location *)
-Lemma partialMonotonicity_assignment :
-  forall σ σ' l C ω ω',
+Lemma pM_assignment :
+  forall σ l C ω ω',
     getObj σ l = Some (C, ω) ->
     length ω <= length ω' ->
-    σ' = [l ↦ (C, ω')]σ ->
-    σ ⪯ σ'.
+    σ ⪯ [l ↦ (C, ω')]σ.
 Proof.
   unfold partialMonotonicity, initializedFields.
   intros.
@@ -88,9 +98,9 @@ Proof.
     rewrite getObj_update1 || rewrite getObj_update2;
     eauto using getObj_dom.
 Qed.
-Global Hint Resolve partialMonotonicity_assignment: pM.
+Global Hint Resolve pM_assignment: pM.
 
-Lemma partialMonotonicity_freshness :
+Lemma pM_freshness :
   forall σ c ρ,
     σ ⪯ σ ++ [(c, ρ)].
 Proof.
@@ -98,51 +108,80 @@ Proof.
   induction σ ; destruct l => //.
   apply IHσ => //.
 Qed.
-Global Hint Resolve partialMonotonicity_freshness: pM.
+Global Hint Resolve pM_freshness: pM.
 
 (** Then we have the main result *)
-Theorem partialMonotonicity_theorem:
-  forall n, forall e σ σ' ρ v v',
-      ⟦e⟧(σ, ρ, v)(n) = Success v' σ' ->
-      σ ⪯ σ'.
-Proof.
-  apply (EvalMaintainedProp partialMonotonicity);
-    try (intros; apply FreshnessInitMaintained);
-    unfoldProps;
-    eauto with pM.
+Theorem pM_theorem:
+  forall e σ σ' ρ ψ v,
+      ⟦e⟧p (σ, ρ, ψ) --> (v, σ') -> σ ⪯ σ'.
+Proof with (eauto with pM updates lia).
+  intros.
+  induction H using evalP_ind2 with
+    (Pl := fun _ σ _ _ _ σ' _ => σ ⪯ σ')
+    (Pin := fun _ _ _ σ σ' _ => σ ⪯ σ');
+    unfold assign, assign_new in *; steps; pM_trans ...
 Qed.
-Global Hint Resolve partialMonotonicity_theorem: pM.
+Global Hint Resolve pM_theorem: pM.
+
+Theorem pM_theorem_list:
+  forall el σ σ' ρ ψ vl,
+      ⟦_ el _⟧p (σ, ρ, ψ) --> (vl, σ') -> σ ⪯ σ'.
+Proof with (eauto with pM updates lia).
+  intros.
+  induction H ...
+Qed.
+Global Hint Resolve pM_theorem_list: pM.
+
+Theorem pM_theorem_init:
+  forall fls ψ ρ σ σ',
+      initP fls ψ ρ σ σ' -> σ ⪯ σ'.
+Proof with (eauto with pM updates lia).
+  intros.
+  induction H;
+    unfold assign, assign_new in *; steps ...
+  eapply pM_theorem in H. pM_trans ...
+Qed.
+Global Hint Resolve pM_theorem_init: pM.
 
 (** ** Other conservation results *)
 (** As a consequence, we have monotonicity on the sizes of stores *)
-Theorem partialMonotonicity_theorem_dom:
-  forall n, forall e σ σ' ρ v v',
-      ⟦e⟧(σ, ρ, v)(n) = Success v' σ' ->
-      dom σ <= dom σ'.
+Lemma evalP_dom:
+   forall e σ ρ ψ v σ',
+      ⟦e⟧p (σ, ρ, ψ) --> (v, σ') -> dom σ <= dom σ'.
 Proof.
   eauto with pM.
 Qed.
-Global Hint Resolve partialMonotonicity_theorem_dom: pM.
+Global Hint Resolve evalP_dom: pM.
+
+Lemma evalListP_dom:
+   forall el σ ρ ψ vl σ',
+      ⟦_ el _⟧p (σ, ρ, ψ) --> (vl, σ') -> dom σ <= dom σ'.
+Proof.
+  eauto with pM.
+Qed.
+Global Hint Resolve evalListP_dom: pM.
+
+Lemma initP_dom:
+  forall fls ψ ρ σ σ',
+      initP fls ψ ρ σ σ' -> dom σ <= dom σ'.
+Proof.
+  eauto with pM.
+Qed.
+Global Hint Resolve initP_dom: pM.
 
 Ltac eval_dom :=
-  match goal with
-  | H: ⟦?e⟧(?σ, ?ρ, ?v)(?n) = Success ?v' ?σ' |- _ =>
+  repeat match goal with
+  | H: ⟦ ?e ⟧p (?σ, ?ρ, ?ψ) --> (?v, ?σ') |- _ =>
     let fresh := fresh "H_dom" in
-    add_hypothesis fresh (partialMonotonicity_theorem_dom n e σ σ' ρ v v' H)
+    add_hypothesis fresh (evalP_dom e σ ρ ψ v σ' H)
+  | H: ⟦_ ?el _⟧p (?σ, ?ρ, ?ψ) --> (?vl, ?σ') |- _ =>
+    let fresh := fresh "H_dom" in
+    add_hypothesis fresh (evalListP_dom el σ ρ ψ vl σ' H)
+  | H: initP ?fls ?ψ ?ρ ?σ ?σ' |- _ =>
+    let fresh := fresh "H_dom" in
+    add_hypothesis fresh (initP_dom fls ψ ρ σ σ' H)
   end.
 
-
-(** Similarly, we have a result for evaluation of lists *)
-Theorem partialMonotonicity_theorem_list_dom:
-  forall n el σ σ' ρ ψ ρ',
-    ⟦_ el _⟧(σ, ρ, ψ)(n) = (Success_l ρ' σ') ->
-    dom σ <= dom σ'.
-Proof.
-  intros.
-  eapply (EvalListMaintained (fun σ σ' => dom σ <= dom σ') (S n));
-    unfoldProps ; eauto with pM lia.
-Qed.
-Global Hint Resolve partialMonotonicity_theorem_list_dom: pM.
 
 (** If we combine partial monotonicity with compatibility (objects do no change type), we can prove that warm objects stay warm *)
 Lemma partialMonotonicity_warm_monotone:
